Try simplifying condition but revert
Attempt to simplify conditions to be 'hi s < lo s' rather
than using stamp_under but introduces dependance on is_IntegerStamp that complicates further

Graph/Stamp.thy
@@ -223,7 +223,7 @@ fun compatible :: "Stamp \<Rightarrow> Stamp \<Rightarrow> bool" where
   "compatible _ _ = False"
 
 fun stamp_under :: "Stamp \<Rightarrow> Stamp \<Rightarrow> bool" where
-  "stamp_under (IntegerStamp b1 lo1 hi1) (IntegerStamp b2 lo2 hi2) = (b1 = b2 \<and> hi1 < lo2)" |
+  "stamp_under (IntegerStamp b1 lo1 hi1) (IntegerStamp b2 lo2 hi2) = (hi1 < lo2)" |
   "stamp_under _ _ = False"
 
 \<comment> \<open>
